monad laws

src/Writer.dfy
@@ -26,8 +26,32 @@ module {:options "-functionSyntax:4"} Writer {
     Writer<T>.Result(f(w.value).value, w.log + f(w.value).log)
   }
 
+  function Composition<S,T,U>(f: S -> Writer<T>, g: T -> Writer<U>): S -> Writer<U> {
+    x => Bind(f(x), g)
+  }
+
   lemma LemmaUnitalityJoin<T>(w: Writer<T>)
     ensures Join(Map(Return<T>)(w)) == w == Join(Return<Writer<T>>(w))
+  {
+  }
+
+  lemma LemmaAssociativityJoin<T>(www: Writer<Writer<Writer<T>>>) 
+    ensures Join(Map(Join<T>)(www)) == Join(Join<Writer<T>>(www))
+  {
+  }  
+
+  lemma LemmaLeftUnitalityBind<S,T>(v: S, f: S -> Writer<T>)
+    ensures Bind(Return(v), f) == f(v)
+  {
+  }
+
+  lemma LemmaRightUnitalityBind<T>(w: Writer<T>)
+    ensures Bind(w, Return) == w
+  {
+  }
+
+  lemma LemmaAssociativityBind<S,T,U>(w: Writer<S>, f: S -> Writer<T>, g: T -> Writer<U>)
+    ensures Bind(Bind(w, f), g) == Bind(w, Composition(f, g))
   {
   }
 
